mostly working cancel_log_rep...

src/ChecksumLog.v
@@ -13,6 +13,7 @@ Require Import GenSep.
 
 Set Implicit Arguments.
 
+
 Definition DataStart : addr := $0.
 Definition HashStart : addr := $1.
 Definition Interval : addr := $2.
@@ -21,6 +22,9 @@ Parameter maxlen : addr.
 Definition list_prefix A (p l : list A) :=
   firstn (length p) l = p.
 
+Definition list_suffix_repeat A (p l : list A) x :=
+  skipn (length p) l = repeat x (length l - length p).
+
 (* TODO: Probably need something about how the next hash block on disk
   doesn't match the current values. *)
 Definition log_rep vl hl (log_pointer : addr) hm vdisk hdisk :
@@ -28,7 +32,8 @@ Definition log_rep vl hl (log_pointer : addr) hm vdisk hdisk :
   (exists unsynced_data unsynced_hashes,
     [[ length vdisk = # (maxlen) /\ length hdisk = # (maxlen) ]] *
     [[ length vl = # (log_pointer) /\ length hl = # (log_pointer) ]] *
-    [[ list_prefix (rev vl) vdisk /\ list_prefix (rev hl) hdisk]] *
+    [[ list_prefix (rev vl) vdisk /\ list_prefix (rev hl) hdisk /\
+        list_suffix_repeat hl hdisk default_hash ]] *
     array DataStart (combine vdisk unsynced_data) Interval *
     [[ length unsynced_data = length vdisk ]] *
     array HashStart (combine (map hash_to_valu hdisk)
@@ -63,6 +68,28 @@ Definition truncate T cs rx : prog T :=
   cs <- BUFCACHE.write_array HashStart $0 Interval (hash_to_valu h) cs;
   rx (cs, natToWord addrlen 0).
 
+
+(* Some list helpers *)
+Lemma skipn_repeat_updN : forall T (a b : T) n n' i l,
+  skipn n l = repeat a n' ->
+  i < n ->
+  skipn n (updN l i b) = repeat a n'.
+Proof.
+Admitted.
+
+
+Lemma skipn_repeat_S : forall A (l : list A) x n n',
+  skipn n l = repeat x (S n') ->
+  skipn (S n) l = repeat x n'.
+Proof.
+  induction l; intros; simpl in *.
+  destruct n; inversion H.
+
+  destruct n; inversion H; auto.
+  eapply IHl. auto.
+Qed.
+
+
 Theorem append_ok : forall log_pointer v cs,
   {< d vl hl,
   PRE:hm
@@ -78,4 +105,233 @@ Theorem append_ok : forall log_pointer v cs,
          log_rep' (v :: vl) (h :: hl) (log_pointer ^+ $1) hm' cs' d')
   >} append v log_pointer cs.
 Proof.
-Admitted.
+  unfold append, log_rep', log_rep.
+  step.
+  - step.
+    assert (Hl3nil: l3 = nil). apply length_nil; auto.
+    assert (Hl4nil: l4 = nil). apply length_nil; auto.
+    rewrite Hl3nil, Hl4nil in *. clear Hl3nil Hl4nil l3 l4.
+    step.
+    step.
+    rewrite combine_length.
+    rewrite min_r; omega.
+
+    step_idtac; eauto.
+    pred_apply; cancel_with eauto.
+    rewrite combine_length, map_length.
+    rewrite min_r; omega.
+    Ltac cancel_log_rep :=
+    try match goal with
+      | [ |- _ * _ =p=> _ * _ ]
+          => unfold upd_prepend;
+              repeat rewrite <- combine_upd; repeat rewrite <- map_upd;
+              eauto; cancel_with eauto
+      | [ |- length _ = _ ] => repeat rewrite length_upd; omega
+      | [ |- S (S (length _)) = _ ] => erewrite wordToNat_plusone; repeat rewrite length_upd; eauto; omega
+      | [ Hlen: length ?l = ?bound, Hinv: _ < ?bound |- context[(upd ?l _ _)] ]
+        => match goal with
+            | [ H: list_prefix nil _ |- list_prefix _ (upd l _ _) ]
+              => unfold list_prefix; destruct l; rewrite <- Hlen in Hinv;
+                  solve [ inversion Hinv; reflexivity ]
+            | [ H: list_prefix _ _ |- list_prefix _ _ ]
+                  => unfold list_prefix in *;
+                    rewrite <- H at 2;
+                    repeat rewrite firstn_app_updN_eq;
+                    unfold upd;
+                    repeat rewrite app_length;
+                    repeat rewrite rev_length; try omega;
+                    try match goal with
+                      | [ H: S (length ?l) = ?len |- context[length ?l] ]
+                        => replace (length l) with (len - 1);
+                            simpl;
+                            replace (len - 1 + 1) with len;
+                            solve [ try rewrite firstn_updN; try reflexivity; try omega |
+                                    try reflexivity; try omega ]
+                    end
+            | [ H: context[list_suffix_repeat _ _ _]
+                |- context[list_suffix_repeat _ _ _] ]
+              =>  unfold list_suffix_repeat in *; destruct l; rewrite <- Hlen in Hinv;
+                  try solve [ inversion Hinv; reflexivity ];
+                  simpl; inversion H;
+                  rewrite repeat_length;
+                  rewrite <- minus_n_O; auto
+              end
+    end.
+
+    step_with idtac cancel_log_rep.
+
+    constructor.
+    eapply hash_list_rep_subset; eauto.
+    eapply hash_list_rep_subset; eauto.
+    econstructor; try econstructor; eauto.
+    rewrite upd_hashmap'_eq; eauto.
+    eapply hashmap_hashes_neq.
+    apply hashmap_get_default.
+    eauto.
+    intros H'; existT_wordsz_neq H'.
+    constructor.
+
+    cancel.
+    apply pimpl_or_r; left. cancel_with cancel_log_rep.
+    repeat (eapply hash_list_prefixes_subset; eauto).
+
+    cancel.
+    apply pimpl_or_r; right. cancel_with cancel_log_rep.
+    constructor.
+    eapply hash_list_rep_subset; eauto.
+    eapply hash_list_rep_subset; eauto.
+    econstructor; try econstructor; eauto.
+    rewrite upd_hashmap'_eq; eauto.
+    eapply hashmap_hashes_neq.
+    apply hashmap_get_default.
+    eauto.
+    intros H'; existT_wordsz_neq H'.
+    constructor.
+
+    all: (cancel;
+    apply pimpl_or_r; left; cancel_with cancel_log_rep;
+    constructor).
+
+  - apply lt_wlt in H as H'.
+    step.
+    rewrite combine_length, map_length.
+    rewrite wordToNat_minus_one; auto.
+    rewrite min_r; omega.
+
+    step.
+    step.
+    rewrite combine_length.
+    rewrite min_r; omega.
+
+    inversion H7.
+    subst.
+    apply neq0_wneq0 in H18.
+    rewrite <- H5 in H18. intuition.
+
+    assert (Hlengthhl: length l4 = length hl + 1).
+      rewrite <- H19.
+      simpl.
+      omega.
+
+    assert (Hhl: sel l0 (log_pointer ^- $1) default_hash = h).
+      unfold sel.
+      erewrite <- selN_firstn.
+      unfold list_prefix in *.
+      rewrite H12.
+      unfold rev. rewrite <- H19.
+      rewrite selN_app2.
+      rewrite rev_length.
+      rewrite wordToNat_minus_one; auto.
+      rewrite <- H15.
+      rewrite Hlengthhl.
+      simpl.
+      rewrite plus_comm.
+      simpl.
+      rewrite <- minus_n_O.
+      rewrite <- minus_diag_reverse. auto.
+      all: try (rewrite rev_length;
+                rewrite wordToNat_minus_one; intuition; omega).
+
+    step_idtac;
+    clear Hlengthhl.
+
+    eauto.
+    pred_apply; cancel_with eauto.
+    rewrite combine_length, map_length.
+    rewrite min_r; omega.
+
+    step_with idtac cancel_log_rep.
+    unfold list_suffix_repeat in *.
+    simpl. rewrite length_upd. Search hl log_pointer.
+    erewrite <- repeat_updN.
+    instantiate (n := S ( S(length hl))).
+    instantiate (l := l0). simpl. eauto.
+    Search repeat.
+    pose H17 as H''.
+    apply skipn_repeat_S; auto. omega.
+
+
+    cancel.
+    apply pimpl_or_r; left. cancel_with cancel_log_rep.
+    admit.
+    cancel.
+    apply pimpl_or_r; right. cancel_with cancel_log_rep.
+    admit.
+
+    Lemma fst_sel_combine : forall A B (l1 : list A) (l2 : list B) i default,
+      fst (sel (combine l1 l2) i default) = sel l1 i (fst default).
+    Proof. Admitted.
+
+    rewrite fst_sel_combine.
+    erewrite sel_map.
+    rewrite hash2valu2hash.
+    subst; reflexivity.
+    rewrite wordToNat_minus_one; intuition; omega.
+
+    erewrite hashmap_get_subset; eauto.
+    erewrite hashmap_get_subset; eauto.
+    rewrite upd_hashmap'_eq.
+    auto.
+
+
+    Lemma fst_sel_combine : forall A B (l1 : list A) (l2 : list B) i default,
+      fst (sel (combine l1 l2) i default) = sel l1 i (fst default).
+    Proof. Admitted.
+
+    rewrite fst_sel_combine.
+    erewrite sel_map.
+    rewrite hash2valu2hash.
+    replace (length hl) with (# (log_pointer) - 1);
+    replace (# (log_pointer) - 1 + 1) with (# (log_pointer)); try omega.
+    eauto.
+    rewrite wordToNat_minus_one; auto; omega.
+
+    Search hash_list_prefixes.
+    constructor.
+    econstructor.
+    solve_hash_list_rep. reflexivity.
+
+    erewrite hashmap_get_subset; eauto.
+    erewrite hashmap_get_subset; eauto.
+    rewrite fst_sel_combine.
+    erewrite sel_map.
+    rewrite hash2valu2hash.
+    rewrite upd_hashmap'_eq.
+    auto.
+
+    inversion H3.
+    unfold upd_hashmap' in *.
+    contradict H21.
+    apply upd_hashmap_neq.
+    unfold hash_safe in H29; intuition.
+
+    rewrite fst_sel_combine in H31.
+    erewrite sel_map in H31.
+    rewrite hash2valu2hash in H31.
+    rewrite H30 in H31.
+    contradict_hashmap_get_default H31 hm.
+    rewrite wordToNat_minus_one; auto; omega.
+
+    rewrite fst_sel_combine in H31.
+    erewrite sel_map in H31.
+    rewrite hash2valu2hash in H31.
+    rewrite H30 in H31.
+    contradict_hashmap_get_default H31 hm.
+    rewrite wordToNat_minus_one; auto; omega.
+    rewrite wordToNat_minus_one; auto; omega.
+
+    constructor.
+    solve_hash_list_rep.
+    repeat (eapply hash_list_prefixes_subset; eauto).
+
+    cancel.
+    apply pimpl_or_r; left.
+    cancel_with cancel_log_rep.
+    Search list_prefix.
+
+    cancel.
+    cancel.
+
+    Grab Existential Variables.
+    all: eauto.
+Qed.
